src/apps/examples.lean
@@ -1,0 +1,15 @@
+import .topo_translation ..K.jump
+
+open nnf
+
+def boom : nnf := dia (and (var 1) (neg 1))
+
+-- #eval is_sat [boom]
+
+-- #check tableau [boom]
+
+def topo_fact_of (φ : nnf) : psum (∀ (α) (tm : topo_model α) s, ¬ topo_force tm s φ) unit :=
+match tableau [φ] with
+| node.closed _ h _ := psum.inl $ not_topo_force_of_unsat h
+| node.open_ _ := psum.inr ()
+end
